Cslib/Computability/Machines/MultiTapeTuring/Routines/Navigation.lean
@@ -27,15 +27,30 @@ public def outOfList {k : ℕ} (i : Fin k) : MultiTapeTM k Char := sorry
 on tape `i`. Only descends if the current element is a `Data.list` with at least `idx` elements,
 otherwise, the `TapeView` is unchanged. -/
 @[simp]
+public lemma toElem_eval_struct_list {k : ℕ} {idx : ℕ} {i : Fin k}
+  {α : Type} [StrEnc α]
+  {views : Fin k → TapeView}
+  (h_some : ((views i).current.bind (StrEnc.fromData : _ → Option (List α))).isSome) :
+  let ds : List α := ((views i).current.bind StrEnc.fromData).get h_some
+  (toElem idx i).eval_struct views = some
+    (Function.update views i
+        (if idx < ds.length then
+          ⟨(views i).data, (views i).path ++ [idx]⟩
+        else views i)) := by sorry
+
+/-- `toElem idx i` moves to the `idx`th element of the `Data.list` currently pointed to
+on tape `i`. Only descends if the current element is a `Data.list` with at least `idx` elements,
+otherwise, the `TapeView` is unchanged. -/
+@[simp]
 public lemma toElem_eval_struct {k : ℕ} {idx : ℕ} {i : Fin k} {views : Fin k → TapeView} :
   (toElem idx i).eval_struct views = some
     (Function.update views i
-      (match (views i).current with
-      | some (Data.list ds) =>
-        if idx < ds.length then
+      (if h_l : (views i).currentList.isSome then
+        if h_i : idx < ((views i).currentList.get h_l).length then
           ⟨(views i).data, (views i).path ++ [idx]⟩
         else views i
-      | _ => views i)) := by sorry
+      else views i)) := by sorry
+
 
 /-- `outOfArg argIdx i` ascends back from the `argIdx`-th element,
     removing it from the end of the path. If the path ends with `argIdx`,
